Some recursors

SubtypeInduction/NatSubtypes.lean
@@ -24,6 +24,8 @@ def OddNumbers := {n : Nat // Odd n}
 
 #Induct_Pred_Recursor Inductive.EvenNumbers
 
+#check Nat.rec
+
 
 def EvenRec
   {motive : EvenNumbers → Prop}
@@ -80,6 +82,8 @@ def AtLeastRec {n : Nat} {motive : (AtLeast n) -> Prop}
 
 end Inductive
 
+#check Nat.succ
+
 namespace Noninductive
 
 def Even : Nat -> Prop :=
@@ -98,4 +102,251 @@ def EvenNumbers.rec.{u} {motive : EvenNumbers → Sort u} (zero : motive EvenNum
   (succ : (n : EvenNumbers) → motive n → motive n.succ) (t : EvenNumbers) :
   motive t := sorry
 
+def OddNumbers.one : OddNumbers := ⟨Nat.zero.succ, rfl⟩
+def OddNumbers.succ (n : OddNumbers) : OddNumbers := ⟨n.val +2, by grind [= Odd]⟩
+
+inductive IsConstructed : OddNumbers -> Type where
+  | base : IsConstructed OddNumbers.one
+  | step (n : OddNumbers) : IsConstructed n -> IsConstructed (OddNumbers.succ n)
+
+def EveryOddIsConstructed : Type := ∀ (n : OddNumbers), IsConstructed n
+
+def ConsProofOdd : (n : OddNumbers) -> IsConstructed n
+  | ⟨0, h⟩ => by contradiction
+  | ⟨1, h⟩ => IsConstructed.base
+  | ⟨k + 2, h⟩ =>
+    have hk : Odd k := by
+      dsimp [Odd] at h ⊢
+      omega
+    have ih : IsConstructed ⟨k, hk⟩ := ConsProofOdd ⟨k, hk ⟩
+    IsConstructed.step ⟨k, hk⟩ ih
+termination_by n => n.val
+
+def AllConsProofOdd : EveryOddIsConstructed :=
+  ConsProofOdd
+
+def OddNumbers.rec.{u} {motive : OddNumbers → Sort u} (start : motive OddNumbers.one)
+  (succ : (n : OddNumbers) → motive n → motive n.succ) (t : OddNumbers) :
+  motive t :=
+    let rec helper (k : Nat) (h : Odd k) : motive ⟨k, h⟩ :=
+    match k, h with
+      | 0, h0 => by
+        dsimp [Odd] at h0
+        omega
+      | 1, _ => start
+      | k' + 2, h2 => by
+        have hk : Odd k' := by
+          dsimp [Odd] at h2 ⊢
+          omega
+        exact succ ⟨k', hk⟩ (helper k' hk)
+    match t with
+      | ⟨k, h⟩ => helper k h
+
+
+def OddNumbers.rec2.{u} {motive : OddNumbers → Sort u} (start : motive OddNumbers.one)
+  (succ : (n : OddNumbers) → motive n → motive n.succ) (t : OddNumbers) :
+  motive t :=
+    let rec read_blueprint {n : OddNumbers} (blueprint : IsConstructed n) : motive n :=
+    match blueprint with
+    | IsConstructed.base => start
+    | IsConstructed.step m bp => succ m (read_blueprint bp)
+  read_blueprint (ConsProofOdd t)
+
+
+theorem lemma2 {n : Nat} (h : Odd n) : n = 1 ∨ ∃ n', Odd n' ∧ n = n' + 2 :=
+  match n with
+  | 0 => by
+    dsimp [Odd] at h
+    omega
+  | 1 => Or.inl rfl
+  | n + 2 => by
+    have hn : Odd n := by
+      dsimp [Odd] at h ⊢
+      omega
+    exact Or.inr ⟨n, hn, rfl⟩
+
+theorem odd_zero_impossible (h : Odd 0) : False := by
+  have h_cases := lemma2 h
+  match h_cases with
+  | Or.inl h_zero_eq_one => contradiction
+  | Or.inr ⟨n', hn', h_zero_eq_succ⟩ => contradiction
+
+theorem odd_prev {n : Nat} (h : Odd (n + 2)) : Odd n := by
+  dsimp [Odd] at h ⊢
+  omega
+
+
+def OddNumbers.rec3.{u} {motive : OddNumbers → Type u} (start : motive OddNumbers.one)
+  (succ : (n : OddNumbers) → motive n → motive n.succ) (t : OddNumbers) : motive t :=
+
+  let Motive' (k : Nat) : Type u :=
+    ((h : Odd k) → motive ⟨k, h⟩) × ((h : Odd (k + 1)) → motive ⟨k + 1, h⟩)
+
+  let rec helper (k : Nat) : Motive' k :=
+    match k with
+    | 0 =>
+      ( fun h => False.elim (odd_zero_impossible h),
+        fun _ => start )
+
+    | n + 1 =>
+      let prev := helper n
+      ( prev.2,
+        fun h_succ_succ => by
+          have hn : Odd n := odd_prev h_succ_succ
+          exact succ ⟨n, hn⟩ (prev.1 hn) )
+
+  (helper t.val).1 t.property
+
+
+inductive IndEven : Type where
+  | zero' : IndEven
+  | succ' : IndEven -> IndEven
+
+def SubToInd (n : EvenNumbers) : IndEven :=
+  match n with
+  | ⟨0, h⟩ => IndEven.zero'
+  | ⟨n + 2, h⟩ =>
+      have hn : Even n := by
+       dsimp [Even] at h ⊢
+       omega
+      IndEven.succ' (SubToInd ⟨n, hn⟩)
+termination_by n.val
+
+def IndToSub (n : IndEven) : EvenNumbers :=
+  match n with
+  | .zero' => ⟨0, rfl⟩
+  | .succ' n' =>
+      let ⟨n, hn⟩ := IndToSub n'
+      have h : (Even (n + 2)) := by
+        dsimp [Even] at hn ⊢
+        omega
+    ⟨n + 2, h⟩
+
+
+theorem IndToSub_left_inv_SubToInd : Function.LeftInverse IndToSub SubToInd :=
+  fun n =>
+    match n with
+      | ⟨0, h⟩ => by
+        apply Subtype.ext
+        simp [SubToInd, IndToSub]
+      | ⟨k + 2, h⟩ => by
+        have hk : Even k := by
+          dsimp [Even] at h ⊢
+          omega
+        have ih := IndToSub_left_inv_SubToInd ⟨k, hk⟩
+        apply Subtype.ext
+        simp [SubToInd, IndToSub, ih]
+termination_by n => n.val
+
+theorem SubToInd_left_inv_IndToSub : Function.LeftInverse SubToInd IndToSub :=
+  fun n =>
+    match n with
+      | .zero' => by
+        unfold IndToSub
+        ---unfold SubToInd    this should work, I don't know why it doesn't
+        sorry
+
+
+      | .succ' m => by
+        have ih := SubToInd_left_inv_IndToSub m
+        unfold IndToSub
+        cases h : IndToSub m
+        expose_names
+        unfold SubToInd
+        dsimp
+        simp
+        rw[h] at ih
+        rw[ih]
+
+
+def EvenNumbers.rec2.{u} {motive : EvenNumbers → Type u} (start : motive EvenNumbers.zero)
+  (succ : (n : EvenNumbers) → motive n → motive n.succ) (t : EvenNumbers) : motive t :=
+    let rec helper (m : IndEven) : motive (IndToSub m) :=
+      match m with
+        | .zero' => by
+          unfold IndToSub
+          apply start
+        | .succ' m => by
+          let ih := helper m
+          unfold IndToSub
+          cases h : IndToSub m
+          dsimp
+          rw [h] at ih
+          expose_names
+          exact succ ⟨val, property⟩ ih
+    by
+      have inv := IndToSub_left_inv_SubToInd t
+      rw [← inv]
+      apply helper (SubToInd t)
+
+
+def mod4_1 : Nat -> Prop :=
+  fun n => n%4 = 1
+
+def mod4_1Number := {n : Nat // mod4_1 n}
+
+def mod4_1Number.one : mod4_1Number := ⟨1, rfl⟩
+def mod4_1Number.succ (n : mod4_1Number) : mod4_1Number := ⟨n.val + 4, by grind [mod4_1]⟩
+
+def mod4_1Number.rec.{u} {motive : mod4_1Number → Type u} (one : motive mod4_1Number.one)
+  (succ : (n : mod4_1Number) → motive n → motive n.succ) (t : mod4_1Number) : motive t :=
+  let Motive' (k : Nat) : Type u :=
+    ((h : mod4_1 k)       → motive ⟨k, h⟩) × ((h : mod4_1 (k + 1)) → motive ⟨k + 1, h⟩) ×
+    ((h : mod4_1 (k + 2)) → motive ⟨k + 2, h⟩) × ((h : mod4_1 (k + 3)) → motive ⟨k + 3, h⟩)
+
+  let rec helper (k : Nat) : Motive' k :=
+    match k with
+      | 0 =>
+        ( fun h => by dsimp [mod4_1] at h; omega,
+          fun _ => one,
+          fun h => by dsimp [mod4_1] at h; omega,
+          fun h => by dsimp [mod4_1] at h; omega )
+      | n + 1 =>
+        let prev := helper n
+        ( prev.2.1,
+          prev.2.2.1,
+          prev.2.2.2,
+          fun h_succ => by
+            have hn : mod4_1 n := by
+              dsimp [mod4_1] at h_succ ⊢
+              omega
+            exact succ ⟨n, hn⟩ (prev.1 hn)
+              )
+
+  (helper t.val).1 t.property
+
+
 end Noninductive
+
+#check Fin
+
+
+#check Fin.rec
+
+#check Fin.induction
+
+def Fin.rec2.{u} {n : Nat} (h : n > 0)
+  {motive : Fin n -> Sort u}
+  (zero : motive ⟨0, h⟩)
+  (succ : (m : Fin (n - 1)) ->
+          motive (Fin.cast (Nat.sub_add_cancel h) m.castSucc) ->
+          motive (Fin.cast (Nat.sub_add_cancel h) m.succ))
+  (i : Fin n) : motive i :=
+    let rec helper (k : Nat) (h : k < n) : motive ⟨k, h⟩ :=
+      match k, h with
+      |0, h => zero
+      |n + 1 , h => by
+        expose_names
+        have hn : n < n_1 - 1 := by omega
+        have h_eq_fin : Fin.cast (Nat.sub_add_cancel h_1) (Fin.succ ⟨n, hn⟩) = ⟨n + 1, h⟩ := by
+          apply Fin.ext
+          rfl
+        have hn_cast : n < n_1 := by omega
+        let rec_call := helper n hn_cast
+        exact h_eq_fin ▸ succ ⟨n, hn⟩ rec_call
+  match i with
+    | ⟨k, h⟩ => helper k h
+
+
+-- it kind of feels like what interesting here is the fact that we can propegate the predicate downwards along the structure of the natural numbers, which allows us
+-- to recurse downwards and stay in the subtype (is that just a recursive predicate and therefore a case of the ornament stuff)
