SubtypeInduction/Multiset_Recursor.lean
@@ -1,0 +1,73 @@
+import Mathlib.Data.List.Sort
+import Mathlib.Data.Multiset.Basic
+import Mathlib.Data.Finset.Basic
+
+def MultisetAsSubtype (α : Type) [LinearOrder α] := { l : List α // List.Pairwise (· ≤ ·) l }
+
+def MultisetAsSubtype.add {α : Type} [LinearOrder α] (a : α) (l : MultisetAsSubtype α) : MultisetAsSubtype α :=
+  let newList := (a :: l.val).mergeSort (fun x y => decide (x ≤ y))
+  have isSorted : newList.Pairwise (· ≤ ·) := List.pairwise_mergeSort' (· ≤ ·) (a :: l.val)
+  ⟨newList, isSorted⟩
+
+#check Multiset
+
+#check Multiset.rec
+
+#check Finset.rec
+
+#check Finset.induction_on
+
+lemma not_in_cons_of_neq {α} (a a' : α) (f : Finset α) (ha : a ∉ f) (ha' : a' ∉ f) (h_neq : a' ≠ a) :
+  a' ∉ Finset.cons a f ha := by
+    intro h_in
+    rcases Multiset.mem_cons.mp h_in with h_eq | h_mem
+    · exact h_neq h_eq
+    · exact ha' h_mem
+
+
+
+def Finset.rec2 {α : Type _} (motive : Finset α -> Sort u) (start : motive ∅)
+  (step : (a : α) → (f : Finset α) -> (h : a ∉ f) -> motive f -> motive (Finset.cons a f h))
+  (comm : ∀ (a a' : α) (f : Finset α) (ha : a ∉ f) (ha' : a' ∉ f) (h_neq : a ≠ a') (b : motive f),
+    step a' (Finset.cons a f ha)
+      (not_in_cons_of_neq a a' f ha ha' h_neq.symm)
+      (step a f ha b)
+    ≍
+    step a (Finset.cons a' f ha')
+      (not_in_cons_of_neq a' a f ha' ha h_neq)
+      (step a' f ha' b)
+  )
+  (t : Finset α) : motive t :=
+   match t with
+    | ⟨s, nd⟩ =>
+      let C : Multiset α → Sort u := fun m => (nd : m.Nodup) → motive ⟨m, nd⟩
+      let C0 : C 0 := fun nd => start
+      let C_cons : (a : α) → (m : Multiset α) → C m → C (a ::ₘ m) := by
+        intro a m cm nd_cons
+        have h_notin := (Multiset.nodup_cons.mp nd_cons).1
+        have h_nodup := (Multiset.nodup_cons.mp nd_cons).2
+        exact step a ⟨m, h_nodup⟩ h_notin (cm h_nodup)
+      let C_cons_heq_body : ∀ (a a' : α) (m : Multiset α) (b : C m)
+            (nd1 : (a ::ₘ a' ::ₘ m).Nodup)
+            (nd2 : (a' ::ₘ a ::ₘ m).Nodup),
+            C_cons a (a' ::ₘ m) (C_cons a' m b) nd1
+            ≍
+            C_cons a' (a ::ₘ m) (C_cons a m b) nd2 := by
+              intro a a' m b nd1 nd2
+              have ⟨h_notin_nd11, h_nodup_nd12⟩ := Multiset.nodup_cons.mp nd1
+              have ⟨h_notin_nd21, h_nodup_nd22⟩ := Multiset.nodup_cons.mp nd2
+              rw [Multiset.mem_cons] at h_notin_nd11
+              push Not at h_notin_nd11
+              rcases h_notin_nd11 with ⟨h_neq, h_notin_m_a⟩
+              have ⟨h_notin_m_a', h_nodup_m⟩ := Multiset.nodup_cons.mp h_nodup_nd12
+              dsimp [C_cons]
+              exact (comm a a' ⟨m, h_nodup_m⟩ h_notin_m_a h_notin_m_a' h_neq (b h_nodup_m)).symm
+      let C_cons_heq : ∀ (a a' : α) (m : Multiset α) (b : C m),
+        C_cons a (a' ::ₘ m) (C_cons a' m b) ≍ C_cons a' (a ::ₘ m) (C_cons a m b) := by
+          intro a a' m b
+          have h_domain : (a ::ₘ a' ::ₘ m).Nodup = (a' ::ₘ a ::ₘ m).Nodup := by
+            rw [Multiset.cons_swap a a' m]
+          refine Function.hfunext h_domain ?_
+          intro nd1 nd2 h_prop
+          exact C_cons_heq_body a a' m b nd1 nd2
+      Multiset.rec C0 C_cons C_cons_heq s nd
